wip

src/matroid/maps/equiv.lean
@@ -11,7 +11,10 @@ universe u
 
 section iso
 
+
+
 variables {E E₀ E₁ E₂ : Type u} {M₀ : matroid E₀} {M₁ : matroid E₁} {M₂ : matroid E₂}
+
 
 /-- Two matroids are isomorphic if there is a map between ground sets that preserves bases -/
 def is_iso (M₁ : matroid E₁) (M₂ : matroid E₂) (e : E₁ ≃ E₂) :=
@@ -30,59 +33,137 @@ instance : has_coe_to_fun (M₁ ≃i M₂) (λ _, E₁ → E₂) :=
 def iso.refl (M : matroid E) : M ≃i M := ⟨equiv.refl E, λ B, by simp⟩
 def iso.symm (e : M₁ ≃i M₂) : M₂ ≃i M₁ := ⟨e.to_fun.symm, λ B, by {rw e.on_base, simp, }⟩
 
-/-- An equivalence between types induces a map from a matroid on one type to one on another -/
-def congr_equiv (M₁ : matroid E₁) (e : E₁ ≃ E₂) : matroid E₂ :=
-{ base := λ B, M₁.base (e ⁻¹' B),
-  exists_base' := by
-    {obtain ⟨B₁,hB₁⟩ := M₁.exists_base, exact ⟨e '' B₁, by simpa using hB₁⟩} ,
-  base_exchange' :=
-  begin
-    rintro B₁ B₂ hB₁ hB₂ x hx,
-    have hx' : e.symm x ∈ e ⁻¹' B₁ \ e⁻¹' B₂, by simpa,
-    obtain ⟨y, hy, hBy⟩ := hB₁.exchange hB₂ hx',
-    refine ⟨e y, by simpa, _⟩,
-    dsimp only,
-    simp_rw [←union_singleton, preimage_union, preimage_diff] at ⊢ hBy,
-    convert hBy;
-    simp [preimage_equiv_eq_image_symm],
-  end,
-  maximality := 
-  begin
-    rintro I X ⟨B, hB, hIB⟩ hIX, 
-    obtain ⟨J, ⟨⟨BJ,hBJ,hBJB⟩,⟨hIJ, hJX⟩⟩, hJmax⟩
-      := M₁.maximality (e ⁻¹' I) (e ⁻¹' X) ⟨e ⁻¹' B, _⟩ (preimage_mono hIX), 
-    { refine ⟨e '' J, ⟨⟨e '' BJ, by simpa, image_subset _ hBJB⟩,_,_⟩, _⟩,  
-      { convert image_subset e hIJ, rw e.image_preimage },
-      { convert image_subset e hJX, rw e.image_preimage },
-      rintro K ⟨⟨BK, hBK, hKBK⟩, hIK, hKX⟩ hJK, 
-      rw [←e.preimage_subset, e.preimage_image], 
-      refine hJmax ⟨⟨_,hBK,preimage_mono hKBK⟩,preimage_mono hIK,preimage_mono hKX⟩ _, 
-      convert preimage_mono hJK, 
-      rw e.preimage_image },
-    exact ⟨hB, preimage_mono hIB⟩,  
-  end }
+end iso 
 
-@[simp] lemma congr_equiv_apply_base {e : E₁ ≃ E₂} {M₁ : matroid E₁} {B : set E₂} :
-  (M₁.congr_equiv e).base B ↔ M₁.base (e ⁻¹' B) :=
-iff.rfl
+section embed
+
+variables {E E' : Type u} {f : E ↪ E'} 
+
+/-- Embed a matroid as a restriction in a larger type. All elements outside the image are loops. -/
+def image (M : matroid E) (f : E ↪ E') : matroid E' :=
+matroid_of_indep (λ I', ∃ I, M.indep I ∧ I' = f '' I) ⟨_, M.empty_indep, by simp⟩
+( begin 
+  rintro _ _ ⟨J, hJ, rfl⟩ hIJ, refine ⟨J ∩ f ⁻¹' I, hJ.subset (inter_subset_left _ _), _⟩,
+  rw [image_inter f.injective, image_preimage_eq_inter_range, ←inter_assoc, 
+    inter_eq_right_iff_subset.mpr hIJ, eq_comm, 
+    inter_eq_left_iff_subset.mpr (hIJ.trans (image_subset_range _ _))], 
+  end)
+( begin
+    rintro _ _ ⟨I, hI, rfl⟩ hIn ⟨⟨B,hB,rfl⟩,hBmax⟩, 
+    obtain ⟨e, he, heI⟩ := hI.exists_insert_of_not_base _ (hB.base_of_maximal (λ J hJ hBJ, _)), 
+    { exact ⟨f e, by rwa [←image_diff f.injective, f.injective.mem_set_image], 
+      ⟨_, heI, image_insert_eq.symm⟩⟩ },
+    { refine λ hI', hIn ⟨⟨_,hI,rfl⟩,_⟩, 
+      rintro _ ⟨J, hJ, rfl⟩ hIJ,  
+      rw hI'.eq_of_subset_indep hJ, 
+      rwa image_subset_image_iff f.injective at hIJ },
+    exact hBJ.antisymm 
+      ((image_subset_image_iff f.injective).mp (hBmax ⟨_,hJ,rfl⟩ (image_subset _ hBJ))),   
+  end)
+(begin
+  rintro _ X ⟨I,hI,rfl⟩ hIX, 
+  obtain ⟨J, hIJ, hJ⟩ := hI.subset_basis_of_subset (image_subset_iff.mp hIX), 
+  refine ⟨f '' J, ⟨⟨_,hJ.indep,rfl⟩,image_subset _ hIJ, image_subset_iff.mpr hJ.subset⟩, _⟩,
+  rintro _ ⟨⟨K,hK,rfl⟩,hIK,hKX⟩ hJK,   
+  rw hJ.eq_of_subset_indep hK ((image_subset_image_iff f.injective).mp hJK) 
+    (image_subset_iff.mp hKX), 
+end)
+
+@[simp] lemma image_indep_iff {I' : set E'} {M : matroid E} : 
+  (M.image f).indep I' ↔ ∃ I, M.indep I ∧ I' = f '' I := 
+by simp [image]
+ 
+
+/-- A matroid on `E'` and an injection from `E` into `E'` gives rise to a matroid on `E` -/
+def preimage {E E' : Type u} (M' : matroid E') (f : E ↪ E') : matroid E := 
+matroid_of_indep (λ I, M'.indep (f '' I)) (by simp) (λ I J hJ hIJ, hJ.subset (image_subset _ hIJ))
+(begin
+  intros I B hI hIn hB,
+  obtain ⟨e, ⟨⟨e,he,rfl⟩,he'⟩ , hi⟩ := 
+    @indep.exists_insert_of_not_basis _ _ _ (f '' B) (range f) hI (image_subset_range _ _) _ _, 
+  { rw [f.injective.mem_set_image] at he', 
+    rw [←image_insert_eq] at hi, 
+    exact ⟨e, ⟨he,he'⟩, hi⟩ },
+  { refine λ hI', hIn ⟨hI,λ J hJ hIJ, ((image_eq_image f.injective).mp _).subset⟩,
+    exact (hI'.eq_of_subset_indep hJ (image_subset _ hIJ) (image_subset_range _ _)).symm },
+  refine hB.1.basis_of_maximal_subset (image_subset_range _ _) (λ J hJ hBJ hJr, _), 
+  obtain ⟨J, rfl⟩ := subset_range_iff_exists_image_eq.mp hJr, 
+  exact image_subset _ (hB.2 hJ ((image_subset_image_iff f.injective).mp hBJ))
+end)
+(begin
+  intros I X hI hIX, 
+  obtain ⟨J, hIJ, hJ⟩ := hI.subset_basis_of_subset (image_subset _ hIX), 
+  obtain ⟨J, rfl⟩ := subset_range_iff_exists_image_eq.mp (hJ.subset.trans (image_subset_range _ _)), 
+  
+  refine ⟨J, ⟨hJ.indep, (image_subset_image_iff f.injective).mp hIJ, 
+    (image_subset_image_iff f.injective).mp hJ.subset⟩, λ K hK hJK, 
+    (image_subset_image_iff f.injective).mp 
+      (hJ.2 ⟨hK.1,image_subset _ hK.2.2⟩ (image_subset _ hJK))⟩,
+end)
+
+@[simp] lemma preimage_indep_iff {M' : matroid E'} {I : set E} :
+  (M'.preimage f).indep I ↔ M'.indep (f '' I) := 
+by simp [preimage]
+  
+@[simp] lemma preimage_image_eq (M : matroid E) (f : E ↪ E') : (M.image f).preimage f = M :=
+begin
+  refine eq_of_indep_iff_indep_forall (λ I, _), 
+  rw [preimage_indep_iff, image_indep_iff], 
+  refine ⟨_,λ h, ⟨_,h,rfl⟩⟩, 
+  rintro ⟨I₀,hI₀, hf⟩, rwa (image_eq_image f.injective).mp hf,
+end 
+
+@[simp] lemma preimage_cl_eq (M : matroid E') (f : E ↪ E') (X : set E) : 
+  (M.preimage f).cl X = f ⁻¹' (M.cl (f '' X)) :=
+begin
+  rw set.ext_iff, 
+  refine λ e, (em (e ∈ X)).elim 
+    (λ heX, iff_of_true (mem_cl_of_mem _ heX) (mem_cl_of_mem M ⟨_, heX, rfl⟩)) 
+    (λ heX, _),  
+  obtain ⟨I, hI⟩ := (M.preimage f).exists_basis X, 
+  
+  have hb : M.basis (f '' I) (f '' X), 
+  { simp_rw [basis_iff, preimage_indep_iff] at hI,  
+    refine indep.basis_of_maximal_subset hI.1 (image_subset _ hI.2.1) (λ J hJ hIJ hJX, _),
+    obtain ⟨J, rfl⟩ := subset_range_iff_exists_image_eq.mp (hJX.trans (image_subset_range _ _)),   
+    rw hI.2.2 J hJ ((image_subset_image_iff f.injective).mp hIJ) 
+      ((image_subset_image_iff f.injective).mp hJX) },
+  rw [←hI.cl, hI.indep.mem_cl_iff_of_not_mem (not_mem_subset hI.subset heX), preimage_indep_iff, 
+    ←hb.cl, mem_preimage, hb.indep.mem_cl_iff_of_not_mem _, image_insert_eq],
+  rw f.injective.mem_set_image, 
+  exact not_mem_subset hI.subset heX,  
+end 
+
+end embed
+
+section congr 
+
+variables {E E₀ E₁ E₂ : Type u} {M₀ : matroid E₀} {M₁ : matroid E₁} {M₂ : matroid E₂}
+
+/-- An equivalence between types induces a map from a matroid on one type to one on another -/
+def congr_equiv (M₁ : matroid E₁) (e : E₁ ≃ E₂) : matroid E₂ := M₁.preimage (e.symm.to_embedding)
 
 @[simp] lemma congr_equiv_apply_indep {e : E₁ ≃ E₂} {M₁ : matroid E₁} {I : set E₂} :
   (M₁.congr_equiv e).indep I ↔ M₁.indep (e ⁻¹' I) :=
-begin
-  simp_rw [indep, congr_equiv_apply_base],
-  split,
-  { rintro ⟨B₂, hB₂, hIB₂⟩, exact ⟨_, hB₂, preimage_mono hIB₂⟩},
-  rintro ⟨B₁, hB₁, hIB₁⟩,
-  refine ⟨e '' B₁, by rwa e.preimage_image, _⟩,
-  rwa [←equiv.subset_image, ←preimage_equiv_eq_image_symm],
-end
-
-@[simp] lemma congr_equiv_apply_symm_base {e : E₁ ≃ E₂} {M₂ : matroid E₂} {B : set E₁} :
-  (M₂.congr_equiv e.symm).base B ↔ M₂.base (e '' B) :=
-by simp [←image_equiv_eq_preimage_symm]
+by simp [congr_equiv, preimage_equiv_eq_image_symm]
 
 @[simp] lemma congr_equiv_apply_symm_indep {e : E₁ ≃ E₂} {M₂ : matroid E₂} {I : set E₁} :
   (M₂.congr_equiv e.symm).indep I ↔ M₂.indep (e '' I) :=
+by simp [←image_equiv_eq_preimage_symm]
+
+@[simp] lemma congr_equiv_apply_base {e : E₁ ≃ E₂} {M₁ : matroid E₁} {B : set E₂} :
+  (M₁.congr_equiv e).base B ↔ M₁.base (e ⁻¹' B) :=
+begin
+  simp only [base_iff_maximal_indep, congr_equiv, preimage_indep_iff, equiv.coe_to_embedding], 
+  simp only [preimage_equiv_eq_image_symm, and.congr_right_iff], 
+  exact λ h, ⟨λ h' I hI hBI, (e.eq_image_iff_symm_image_eq _ _).mp 
+    (h' _ (by rwa [e.symm_image_image]) ((e.subset_image _ _).mp hBI)), 
+    λ h' I hI hBI, (e.symm.image_eq_iff_eq _ _).mp (h' _ hI (image_subset _ hBI))⟩,   
+end 
+
+
+@[simp] lemma congr_equiv_apply_symm_base {e : E₁ ≃ E₂} {M₂ : matroid E₂} {B : set E₁} :
+  (M₂.congr_equiv e.symm).base B ↔ M₂.base (e '' B) :=
 by simp [←image_equiv_eq_preimage_symm]
 
 @[simp] lemma congr_equiv_apply_basis {e : E₁ ≃ E₂} {M₁ : matroid E₁} {I X : set E₂} :
@@ -133,7 +214,7 @@ begin
   { convert h (e.symm x) (by simpa),
     rw [←image_singleton, preimage_equiv_eq_image_symm]},
   convert h _ hx,
-  rw [←image_singleton, preimage_image_eq _ e.injective],
+  rw [←image_singleton, set.preimage_image_eq _ e.injective],
 end
 
 @[simp] lemma congr_equiv_apply_symm_circuit {e : E₁ ≃ E₂} {M₂ : matroid E₂} {C : set E₁} :
@@ -154,73 +235,9 @@ end
   (M₂.congr_equiv e.symm).flat F = M₂.flat (e '' F) :=
 by simp [←image_equiv_eq_preimage_symm]
 
-end iso
+end congr 
 
-section embed
 
-variables {E E' : Type*} {f : E ↪ E'} 
 
-/-- Embed a matroid as a restriction in a larger type. All elements outside the image are loops. -/
-def image (M : matroid E) (f : E ↪ E') : matroid E' :=
-matroid_of_indep (λ I', ∃ I, M.indep I ∧ I' = f '' I) ⟨_, M.empty_indep, by simp⟩
-( begin 
-  rintro _ _ ⟨J, hJ, rfl⟩ hIJ, refine ⟨J ∩ f ⁻¹' I, hJ.subset (inter_subset_left _ _), _⟩,
-  rw [image_inter f.injective, image_preimage_eq_inter_range, ←inter_assoc, 
-    inter_eq_right_iff_subset.mpr hIJ, eq_comm, 
-    inter_eq_left_iff_subset.mpr (hIJ.trans (image_subset_range _ _))], 
-  end)
-( begin
-    rintro _ _ ⟨I, hI, rfl⟩ hIn ⟨⟨B,hB,rfl⟩,hBmax⟩, 
-    obtain ⟨e, he, heI⟩ := hI.exists_insert_of_not_base _ (hB.base_of_maximal (λ J hJ hBJ, _)), 
-    { exact ⟨f e, by rwa [←image_diff f.injective, f.injective.mem_set_image], 
-      ⟨_, heI, image_insert_eq.symm⟩⟩ },
-    { refine λ hI', hIn ⟨⟨_,hI,rfl⟩,_⟩, 
-      rintro _ ⟨J, hJ, rfl⟩ hIJ,  
-      rw hI'.eq_of_subset_indep hJ, 
-      rwa image_subset_image_iff f.injective at hIJ },
-    exact hBJ.antisymm 
-      ((image_subset_image_iff f.injective).mp (hBmax ⟨_,hJ,rfl⟩ (image_subset _ hBJ))),   
-  end)
-(begin
-  rintro _ X ⟨I,hI,rfl⟩ hIX, 
-  obtain ⟨J, hIJ, hJ⟩ := hI.subset_basis_of_subset (image_subset_iff.mp hIX), 
-  refine ⟨f '' J, ⟨⟨_,hJ.indep,rfl⟩,image_subset _ hIJ, image_subset_iff.mpr hJ.subset⟩, _⟩,
-  rintro _ ⟨⟨K,hK,rfl⟩,hIK,hKX⟩ hJK,   
-  rw hJ.eq_of_subset_indep hK ((image_subset_image_iff f.injective).mp hJK) 
-    (image_subset_iff.mp hKX), 
-end)
-
-@[simp] lemma image_indep_iff {I' : set E'} {M : matroid E} : 
-  (M.image f).indep I' ↔ ∃ I, M.indep I ∧ I' = f '' I := 
-by simp [image]
-
-/-- A matroid on `E'` and an injection from `E` into `E'` gives rise to a matroid on `E` -/
-def preimage {E E' : Type*} (M' : matroid E') (f : E ↪ E') : matroid E := 
-matroid_of_indep (λ I, M'.indep (f '' I)) (by simp) (λ I J hJ hIJ, hJ.subset (image_subset _ hIJ))
-(begin
-  intros I B hI hIn hB,
-  obtain ⟨e, ⟨⟨e,he,rfl⟩,he'⟩ , hi⟩ := 
-    @indep.exists_insert_of_not_basis _ _ _ (f '' B) (range f) hI (image_subset_range _ _) _ _, 
-  { rw [f.injective.mem_set_image] at he', 
-    rw [←image_insert_eq] at hi, 
-    exact ⟨e, ⟨he,he'⟩, hi⟩ },
-  { refine λ hI', hIn ⟨hI,λ J hJ hIJ, ((image_eq_image f.injective).mp _).subset⟩,
-    exact (hI'.eq_of_subset_indep hJ (image_subset _ hIJ) (image_subset_range _ _)).symm },
-  refine hB.1.basis_of_maximal_subset (image_subset_range _ _) (λ J hJ hBJ hJr, _), 
-  obtain ⟨J, rfl⟩ := subset_range_iff_exists_image_eq.mp hJr, 
-  exact image_subset _ (hB.2 hJ ((image_subset_image_iff f.injective).mp hBJ))
-end)
-(begin
-  intros I X hI hIX, 
-  obtain ⟨J, hIJ, hJ⟩ := hI.subset_basis_of_subset (image_subset _ hIX), 
-  obtain ⟨J, rfl⟩ := subset_range_iff_exists_image_eq.mp (hJ.subset.trans (image_subset_range _ _)), 
-  
-  refine ⟨J, ⟨hJ.indep, (image_subset_image_iff f.injective).mp hIJ, 
-    (image_subset_image_iff f.injective).mp hJ.subset⟩, λ K hK hJK, 
-    (image_subset_image_iff f.injective).mp 
-      (hJ.2 ⟨hK.1,image_subset _ hK.2.2⟩ (image_subset _ hJK))⟩,
-end)
-
-end embed
 
 end matroid 
